iris/SpecProcinit.v
@@ -267,7 +267,7 @@ Section ProcinitProcsInv.
   Lemma procs_inv_alloc (E : coPset) :
     ([∗ list] i ∈ seq 0 NPROC,
        ((proc_ready i ∗ (∃ ch : mword 64, p_chan (proc_addr i) ↦₈ ch) ∗
-         proc_pub (proc_addr i)) ∗ (∃ h : CPU, hart_full i h)) ∗
+         proc_pub (proc_addr i)) ∗ hart_full i (0%fin : CPU)) ∗
        pstate_full i UNUSED)
     ={E}=∗ ∃ γs : list gname, procs_inv γs.
   Proof.
@@ -275,16 +275,15 @@ Section ProcinitProcsInv.
     (* 1. peel [lk_fresh] out of each [proc_ready] *)
     iDestruct (big_sepL_impl
                  (fun _ i => (((proc_ready i ∗ (∃ ch : mword 64, p_chan (proc_addr i) ↦₈ ch) ∗
-                                proc_pub (proc_addr i)) ∗ (∃ h : CPU, hart_full i h)) ∗
+                                proc_pub (proc_addr i)) ∗ hart_full i (0%fin : CPU)) ∗
                               pstate_full i UNUSED)%I)
                  (fun _ i => (lk_fresh (proc_addr i) "proc"%string ∗ proc_res i)%I)
                  (seq 0 NPROC) with "Hin []") as "Hin".
     { iIntros "!>" (k i Hk) "(((Hrdy & Hch & Hpub) & Hpark) & Hg)".
       apply lookup_seq in Hk. destruct Hk as [-> Hlt].
       iDestruct "Hch" as (ch) "Hch".
-      iDestruct "Hpark" as (hb) "Hpark".
       iApply (proc_ready_split with "Hrdy Hch Hpub [Hpark] [Hg]").
-      { iApply (hart_at_any_intro k hb Hlt with "Hpark"). }
+      { iApply (hart_at_any_intro k (0%fin : CPU) Hlt with "Hpark"). }
       (* UNUSED is [unclaimed], so the whole variable is the lock's share *)
       rewrite /pstate_lock unclaimed_UNUSED.
       iDestruct (pstate_split k UNUSED with "Hg") as "[Hg1 Hg2]".
